proof/AdequacySound.v
@@ -1,0 +1,161 @@
+Require Import CoqlibC.
+Require Import Simulation.
+Require Import LinkingC.
+Require Import Skeleton.
+Require Import Values.
+Require Import JMeq.
+Require Import Smallstep.
+Require Import Integers.
+Require Import Events.
+
+Require Import Skeleton ModSem Mod Sem.
+Require Import SimSymb SimMem SimMod SimModSem SimProg (* SimLoad *) SimProg.
+Require Import SemProps Ord.
+Require Import Sound Preservation.
+
+Set Implicit Arguments.
+
+
+
+
+Section ADQSOUND.
+
+  Context `{SM: SimMem.class}.
+  Context {SS: SimSymb.class SM}.
+  Context `{SU: Sound.class}.
+
+  Variable pp: ProgPair.t.
+  Hypothesis SIMPROG: ProgPair.sim pp.
+  Let p_src := pp.(ProgPair.src).
+  Let p_tgt := pp.(ProgPair.tgt).
+
+  Variable sk_link_src sk_link_tgt: Sk.t.
+  Hypothesis LINKSRC: (link_sk p_src) = Some sk_link_src.
+  Hypothesis LINKTGT: (link_sk p_tgt) = Some sk_link_tgt.
+  Let sem_src := Sem.sem p_src.
+  Let sem_tgt := Sem.sem p_tgt.
+
+  Let skenv_link_src := sk_link_src.(Sk.load_skenv).
+  Let skenv_link_tgt := sk_link_tgt.(Sk.load_skenv).
+
+  (* stack can go preservation when su0 is given *)
+  Inductive sound_stack (su0: Sound.t): list Frame.t -> Prop :=
+  | sound_stack_nil
+    :
+      sound_stack su0 []
+  | sound_stack_cons
+      su_tail
+      ms lst0 tail
+      (TL: sound_stack su_tail tail)
+      (HD: forall
+          sound_state_all
+          (PRSV: local_preservation ms sound_state_all)
+        ,
+          (<<SUST: sound_state_all su0 lst0>>)
+          /\
+          (<<K: forall
+              retv lst1
+              args
+              (SURETV: Sound.retv su0 retv)
+              (MLE: Sound.mle su0 args.(Args.m) retv.(Retv.m))
+              (AFTER: ms.(ModSem.after_external) lst0 retv lst1)
+            ,
+              sound_state_all su_tail lst1>>)
+      )
+      (* sound_state_ex *)
+      (* (PRSV: local_preservation ms sound_state_ex) *)
+      (* (HD: sound_state_ex su0 lst0) *)
+    :
+      sound_stack su0 ((Frame.mk ms lst0) :: tail)
+  .
+
+  Inductive sound_state (su0: Sound.t): state -> Prop :=
+  | sound_state_normal
+      su_tail ms lst0 tail
+      (TL: sound_stack su_tail tail)
+      (HD: forall
+          sound_state_all
+          (PRSV: local_preservation ms sound_state_all)
+        ,
+          <<SUST: sound_state_all su0 lst0>>)
+    :
+      sound_state su0 (State ((Frame.mk ms lst0) :: tail))
+  | sound_state_call
+      su_tail frs
+      (STK: sound_stack su_tail frs)
+      args
+      (ARGS: Sound.args su0 args)
+    :
+      sound_state su0 (Callstate args frs)
+  .
+
+  Lemma sound_init
+        st0
+        (INIT: sem_src.(Smallstep.initial_state) st0)
+    :
+      exists su0, sound_state su0 st0
+  .
+  Proof.
+    inv INIT.
+    esplits; eauto. econs; eauto.
+    - econs; eauto.
+    - eapply Sound.top_args.
+  Unshelve.
+    all: exact Sound.top.
+  Qed.
+
+  Lemma sound_progress
+        su0 st0 tr st1
+        (SUST: sound_state su0 st0)
+        (STEP: Step sem_src st0 tr st1)
+    :
+      <<SUST: exists su1, sound_state su1 st1>>
+  .
+  Proof.
+    inv STEP.
+    - (* CALL *)
+      inv SUST. ss.
+      assert(exists su_greatest, su_greatest.(Sound.args) args).
+      { admit "". }
+      des.
+      exists su_greatest. econs; eauto. econs; eauto.
+      ii.
+      dsplits; eauto.
+      inv PRSV. exploit CALL; eauto. i; des.
+      assert(su_lifted = su_greatest).
+      { admit "". }
+      clarify.
+      ii. inv PRSV.
+      dup PRSV. inv PRSV. dsplits; eauto. i. exploit CALL; eauto. i; des.
+    - (* INIT *)
+      inv SUST. ss. des_ifs.
+      inv STK.
+      { esplits; eauto. econs; eauto. econs; eauto.
+        - econs; eauto.
+        - ii. inv PRSV. dsplits; eauto.
+          + ii.
+            (* exploit CALL; eauto. *)
+            admit "".
+      }
+      esplits; eauto. econs; eauto. econs; eauto.
+      { econs; eauto. }
+      i. inv PRSV. dsplits; eauto.
+      ii. exploit CALL; eauto.
+    - (* INTERNAL *)
+      inv SUST. inv STK. ss.
+      esplits; eauto.
+      econs; eauto.
+      econs; eauto.
+      ss.
+      ii. dup PRSV. inv PRSV. eapply STEP; eauto.
+      + eapply HD; eauto.
+      + split; ii; ModSem.tac.
+    - (* RETURN *)
+      inv SUST. inv STK. inv TL.
+      esplits; eauto. econs; eauto. econs; eauto. ss.
+      assert(RETV: Sound.retv su0 retv).
+      { admit "". }
+      i. dup PRSV. inv PRSV.
+  Qed.
+
+End ADQSOUND.
