proof/SoundStatePreservation.v
@@ -1,0 +1,420 @@
+
+
+Section SOUNDLPRESSBASE.
+
+
+  Variable ms: ModSem.t.
+  Context `{SU: Sound.class}.
+  Variable sound_state_base: Sound.t -> ms.(ModSem.state) -> Prop.
+  Hypothesis FIN: forall args, Finite {su0 : Sound.t | Sound.args su0 args}.
+  (* Variable sound_state_base_at: forall *)
+  (*     (su_at su_arg: Sound.t) (st: ms.(ModSem.state)) *)
+  (*   , *)
+  (*     Prop *)
+  (* . *)
+
+  (* Context `{FSL: FSL.class Sound.t Sound.le Sound.lub}. *)
+
+  Let get_mem := ms.(ModSem.get_mem).
+
+  Hypothesis INITSOUND: forall
+      args su st0
+      (ARGS: Sound.args su args)
+      (INIT: ms.(ModSem.initial_frame) args st0)
+    ,
+      (<<SS: sound_state_base su st0>>) /\ (<<MLE: Sound.mle su args.(Args.m) st0.(get_mem)>>)
+  .
+
+  Inductive lifted (su_lifted: Sound.t) (args: Args.t): Prop :=
+  | lifted_intro
+      (ARGS: su_lifted.(Sound.args) args)
+  .
+
+  Hypothesis ATSOUND: forall
+      su st0 args
+      (SS: sound_state_base su st0)
+      (AT: ModSem.at_external ms st0 args)
+    ,
+      (<<MLE: Sound.mle su st0.(get_mem) args.(Args.m)>>) /\
+      exists su_lifted, (<<LE: Sound.le su su_lifted>>)
+                        /\ (<<ARGS: su_lifted.(Sound.args) args>>)
+                        (* /\ (<<SUAT: sound_state_base_at su su_lifted st0>>) *)
+  .
+
+  Hypothesis AFTERSOUND: forall
+      su st0 retv su_g st1 args
+      (SS: sound_state_base su st0)
+      (RETV: Sound.retv su_g retv)
+      (LE: Sound.le su su_g)
+      (MLE: Sound.mle su_g args.(Args.m) retv.(Retv.m))
+      (AFTER: ms.(ModSem.after_external) st0 retv st1)
+
+      (GREATEST: forall su_lifted (ARGS: su_lifted.(Sound.args) args), <<LE: Sound.le su_lifted su_g>>)
+      (HISTORY: ms.(ModSem.at_external) st0 args)
+    ,
+      <<SS: sound_state_base su st1>> /\ <<MLE: Sound.mle su retv.(Retv.m) st1.(get_mem)>>
+  .
+
+  Hypothesis FINALSOUND: forall
+      su st0 retv
+      (SS: sound_state_base su st0)
+      (FINAL: ms.(ModSem.final_frame) st0 retv)
+    ,
+      <<RETV: Sound.retv su retv>> /\ <<MLE: Sound.mle su st0.(get_mem) retv.(Retv.m)>>
+  .
+
+  Hypothesis STEPSOUND: forall
+      su st0 tr st1
+      (SS: sound_state_base su st0)
+      (STEP: ms.(ModSem.step) ms.(ModSem.globalenv) st0 tr st1)
+    ,
+      <<SS: sound_state_base su st1>> /\ <<MLE: Sound.mle su st0.(get_mem) st1.(get_mem)>>
+  .
+
+  Lemma sound_state_base_lpres_aux
+        su st0 m_init
+        (SS: sound_state_base su st0)
+        (MLE: Sound.mle su m_init st0.(get_mem))
+    :
+      <<LPRES: lpres ms m_init su st0>>
+  .
+  (* Let sound_state_lpres_aux: forall *)
+  (*       su st0 m_init *)
+  (*       (SS: sound_state su st0) *)
+  (*       (MLE: Sound.mle su m_init st0.(get_mem)) *)
+  (*   , *)
+  (*     <<LPRES: lpres ms m_init su st0>> *)
+  (* . *)
+  Proof.
+    revert_until STEPSOUND.
+    pcofix CIH.
+    i.
+    pfold.
+    destruct (classic (ModSem.is_call ms st0)).
+    {
+      r in H. des.
+      exploit ATSOUND; eauto. i; des.
+      generalize (Sound.refined_FSL args); i.
+      assert(INHAB: exists (su_lifted_refined: {su : Sound.t | Sound.args su args}), su_lifted_refined$ = su_lifted).
+      { unshelve eexists (exist _ su_lifted _).
+        - s. unshelve eauto.
+        - s. unshelve eauto.
+      }
+      exploit (@FSL.find_greatest _ _ _ H0 (fun su => (su $).(Sound.args) args)); eauto.
+      (* set (FSL := Sound.refined_FSL args). *)
+      (* exploit (@FSL.find_greatest _ _ _ FSL (fun su => su.(Sound.args) args)); eauto. *)
+      { ii. eapply Sound.refined_lub_args; eauto. }
+      { des. exists su_lifted_refined. eauto with congruence. }
+      i; des. destruct max as [su_greatest ARGS0].
+      assert(Sound.le su_lifted su_greatest).
+      { rr in MAX. ss. des. specialize (MAX0 su_lifted_refined). rp; [eapply MAX0|..]; eauto with congruence. }
+      eapply lpres_at_external with (su_lifted := su_greatest); eauto.
+      { etrans; eauto. }
+      ii. exploit AFTERSOUND; eauto.
+      { etrans; eauto. }
+      { i. rr in MAX. des. ss.
+        rp; [eapply MAX0|..]; eauto.
+        - unshelve instantiate (1:= exist _ su_lifted0 _); ss.
+        - ss.
+      }
+      i; des.
+      right. eapply CIH; eauto.
+      etrans; eauto.
+      etrans; eauto.
+      etrans; eauto.
+      eapply Sound.le_spec; eauto.
+      etrans; eauto.
+    }
+    destruct (classic (ModSem.is_return ms st0)).
+    {
+      r in H0. des.
+      exploit FINALSOUND; eauto. i; des.
+      econs 3; eauto.
+      etrans; eauto.
+    }
+    econs; eauto.
+    ii. hexpl STEPSOUND. right. eapply CIH; eauto. etrans; eauto.
+  Qed.
+
+  Theorem sound_state_base_lpres
+          args su st0
+          (ARGS: Sound.args su args)
+          (INIT: ms.(ModSem.initial_frame) args st0)
+    :
+      <<LPRES: lpres ms args.(Args.m) su st0>>
+  .
+  Proof.
+    hexpl INITSOUND.
+    eapply sound_state_base_lpres_aux; eauto.
+  Qed.
+
+End SOUNDLPRESSBASE.
+
+
+
+
+
+
+
+Require Import RTLC.
+Require Import ValueDomain ValueAnalysis.
+Require Import Linking.
+
+Variable prog: RTL.program.
+Variable skenv_link: SkEnv.t.
+Let ms := RTLC.modsem skenv_link prog.
+
+
+(* Remark: if econs/econsr gives different goal, at least 2 econs is possible *)
+Ltac econsr :=
+  first
+    [
+    econstructor 16
+    |econstructor 15
+    |econstructor 14
+    |econstructor 13
+    |econstructor 12
+    |econstructor 11
+    |econstructor 10
+    |econstructor  9
+    |econstructor  8
+    |econstructor  7
+    |econstructor  6
+    |econstructor  5
+    |econstructor  4
+    |econstructor  3
+    |econstructor  2
+    |econstructor  1
+    ]
+.
+
+Local Existing Instance Reach.
+
+Definition bc2su (bound: block) (bc: block_classification): t' :=
+  Top.mk (fun blk => bc blk = BCinvalid) bound
+.
+
+Lemma pmatch_sound
+      bc bound blk ofs isreal aptr
+      (PM: pmatch bc blk ofs isreal aptr)
+      (BOUND: Plt blk bound)
+  :
+    <<SU: Sound.val bc.(bc2su bound) (Vptr blk ofs isreal)>>
+.
+Proof.
+  ii; clarify. unfold bc2su; s. esplits; eauto.
+  inv PM; eauto with congruence.
+Qed.
+
+Lemma vmatch_sound
+      bc bound v av
+      (VM: vmatch bc v av)
+      (BOUND: forall blk ofs isreal bound (PTR: v = Vptr blk ofs isreal), Plt blk bound)
+  :
+    <<SU: Sound.val bc.(bc2su bound) v>>
+.
+Proof.
+  inv VM; ss; eapply pmatch_sound; eauto.
+Qed.
+
+Local Transparent Mem.loadbytes.
+Lemma smatch_sound
+      bc bound m bpub aptr
+      (BELOW: bc_below bc bound)
+      (SM: smatch bc m bpub aptr)
+      ofs
+      (PERM : Mem.perm m bpub ofs Cur Readable)
+  :
+    <<SU: memval' bc.(bc2su bound) (ZMap.get ofs (Mem.mem_contents m) !! bpub)>>
+.
+Proof.
+  inv SM.
+  ii; clarify.
+  assert(RPERM: Mem.range_perm m bpub ofs (ofs + 1) Cur Readable).
+  { ii. assert(ofs1 = ofs) by xomega. clarify. }
+  (* exploit (Mem.range_perm_loadbytes m bpub ofs 1); eauto. *)
+  (* { ii. assert(ofs1 = ofs) by xomega. clarify. } *)
+  (* i; des. *)
+  exploit (H0 ofs); eauto.
+  { unfold Mem.loadbytes. des_ifs. ss. rewrite PTR. eauto. }
+  i.
+  assert(bc blk <> BCinvalid).
+  { inv H1; eauto with congruence. }
+  assert(Plt blk bound).
+  { eauto. }
+  s. esplits; eauto.
+Qed.
+
+Lemma mmatch_sound
+      bc m am
+      (MM: mmatch bc m am)
+  :
+    <<SU: Sound.mem bc.(bc2su m.(Mem.nextblock)) m>>
+.
+Proof.
+  inv MM; ss.
+  econs; cycle 1.
+  { ss. refl. }
+  i; clarify.
+  rename blk into bpub. (* rename blk0 into bpriv. *)
+  specialize (mmatch_top bpub).
+  ss. hexploit mmatch_top; eauto. i.
+  eapply smatch_sound; eauto.
+Qed.
+
+Theorem VA_sound_state_base_lpres_aux
+        args su st0
+        (ARGS: Sound.args su args)
+        (INIT: ms.(ModSem.initial_frame) args st0)
+  :
+    lpres ms args.(Args.m) su st0
+.
+Proof.
+  eapply sound_state_base_lpres with (sound_state_base := sound_state_base prog ms.(globalenv)); eauto; ii; ss.
+  - admit "init".
+    (* inv INIT0. esplits; eauto. *)
+    (* + econs; ss; eauto. *)
+  - inv AT; inv SS; ss.
+    split; [r; refl|].
+    exists bc.(bc2su m0.(Mem.nextblock)).
+    hexpl sound_stack_sound_compat COMPAT. inv COMPAT.
+    esplits; eauto.
+    { rr. ii. esplits; eauto. }
+    + econs; ss; eauto.
+      * ii; clarify. inv GE. unfold block in *. spc H1. exploit H1; eauto.
+        { admit "ez". }
+        i; des. rr in H. des; ss.
+      * rewrite Forall_forall. i. eapply vmatch_sound; eauto.
+      * eapply mmatch_sound; eauto.
+  - inv AFTER. ss.
+    des.
+    assert(args0.(Args.m) = m_arg /\ args0.(Args.vs) = vs_arg).
+    { inv HISTORY; ss. }
+    clear HISTORY.
+    des; clarify.
+    inv SS.
+    hexpl sound_stack_sound_compat COMPAT. inv COMPAT.
+    esplits; eauto; try refl.
+    assert(GLE: bc2su (Mem.nextblock (Args.m args0)) bc <1= su_g).
+    { eapply GREATEST. econs; ss; eauto.
+      - admit "history".
+      - rewrite Forall_forall. i. eapply vmatch_sound. eapply ARGS0; eauto.
+      - eapply mmatch_sound; eauto.
+    }
+    inv RETV.
+    set (F := fun blk =>
+                if plt blk args0.(Args.m).(Mem.nextblock)
+                then bc blk
+                else
+                  if plt blk retv.(Retv.m).(Mem.nextblock)
+                  then BCother
+                  else BCinvalid).
+    assert(exists (bc': block_classification), <<IMG: bc'.(bc_img) = F>>).
+    { unshelve eexists (BC _ _ _); ss; eauto.
+      - unfold F. ii. des_ifs. eapply bc_stack; eauto.
+      - unfold F. ii. des_ifs. eapply bc_glob; eauto.
+    } des.
+    eapply sound_return_state with (bc := bc'); ss; eauto.
+    (* econs; ss; eauto. *)
+    + eapply sound_stack_new_bound.
+      { eapply sound_stack_exten with (bc:=bc); eauto.
+        - eapply sound_stack_ext; eauto.
+          ii. inv MLE.
+          erewrite <- Mem.loadbytes_unchanged_on_1; try apply PRIV0; eauto.
+          ii. rr. eapply GLE; ss.
+        - ii. rewrite IMG. unfold F. des_ifs.
+      }
+      inv MLE. ss.
+    + clear - MM IMG F GLE VAL. destruct (Retv.v retv); ss; econs; eauto. destruct b0; ss; econs; eauto.
+      rr in VAL. ii. hexpl VAL. eapply GLE. rr. rewrite IMG in *. unfold F in H. des_ifs. esplits; eauto.
+      { rewrite IMG in *. unfold F in *. des_ifs. 
+      inv MM. eapply mmatch_below; eauto.
+      hexploit VAL; ss; eauto. eapply GLE; eauto.
+      eapply 
+        ttttttttttttttttt
+        eapply LE; eauto.
+        eapply Mem.loadbytes_unchanged_on; eauto.
+        eapply Mem.loadbytes_unchanged_on_1; eauto.
+      }
+      econs; ss; eauto.
+    destruct (pincl (am_nonstack am) Nonstack &&
+                    forallb (fun av => vpincl av Nonstack) aargs)
+             eqn: NOLEAK.
+
+    econs; ss; eauto.
+Qed.
+
+Theorem VA_sound_state_lpres_aux
+        m_init su st0
+        (MLE: Sound.mle su m_init st0.(get_mem))
+        (SS: sound_state prog ms.(globalenv) su st0)
+  :
+    lpres ms m_init su st0
+.
+Proof.
+  eapply sound_state_lpres_aux with (sound_state := sound_state prog ms.(globalenv)); eauto.
+  - ii. ss.
+    inv SS0. inv AT; ss.
+    esplits; eauto.
+    + specialize (H prog (linkorder_refl _)). inv H; ss.
+      assert(FPTR: vmatch bc fptr_arg Vtop).
+      {
+        des.
+        unfold Genv.find_funct in *. des_ifs_safe.
+        econsr. Undo. econs.
+        econsr. Undo. econs.
+        eapply GE. s.
+        admit "ez".
+      }
+      hexpl sound_stack_sound_compat CPT. inv CPT.
+      assert(VTOS: forall v, vmatch bc v Vtop -> su0.(Sound.val) v).
+      { u. ii; clarify. exploit match_aptr_of_aval; eauto. intro P. inv P. eauto. }
+      econs; ss; eauto.
+      * admit "EZ".
+      * econs. ii. clarify; ss.
+        (* PTR: lookup public gives private. *)
+        inv MM.
+        destruct (classic (bc blk = BCinvalid)).
+        { 
+        specialize (mmatch_top blk). exploit mmatch_top; eauto.
+        { ii. eapply inv H. clarify.
+Qed.
+
+
+Theorem VA_sound_state_lpres
+        args su st0
+        (ARGS: Sound.args su args)
+        (INIT: ms.(ModSem.initial_frame) args st0)
+        (SS: sound_state prog ms.(globalenv) su st0)
+  :
+    lpres ms args.(Args.m) su st0
+.
+Proof.
+  eapply sound_state_lpres with (sound_state := sound_state prog ms.(globalenv)); eauto.
+  - ii. inv INIT0.
+    esplits; eauto.
+    + econs; eauto.
+      ii.
+
+      econs; eauto.
+
+  destruct 1.
+  exploit initial_mem_matches; eauto. intros (bc & GE & BELOW & NOSTACK & RM & VALID).
+  constructor; intros. apply sound_call_state with bc.
+- constructor.
+  econs; ii; ss; eauto.
+- simpl; tauto.
+- apply RM; auto.
+- assert(CTX: Val.meminj_ctx).
+  { apply Val.mi_normal. }
+  apply mmatch_inj_top with m0.
+  replace (inj_of_bc bc) with (Mem.flat_inj (Mem.nextblock m0)).
+  eapply Genv.initmem_inject; eauto.
+  symmetry; apply extensionality; unfold Mem.flat_inj; intros x.
+  destruct (plt x (Mem.nextblock m0)).
+  apply inj_of_bc_valid; auto.
+  unfold inj_of_bc. erewrite bc_below_invalid; eauto.
+- exact GE.
+- exact NOSTACK.
+
+Qed.
